Merge from development branch (v4.18.0) (#2)
* Add MePo

* Fix bug argument too long

* Bump to v4.16.0

* Fix naming conflict to ImportGraph

* add python code

* support adding premise

* rename

* rename

* add warning

* small refactor

* dedup added modules

* gitignore DS_Store

* view added premises

* Update links

* Update links

* add blacklisted premises to unfiltered_premises

* refactor server to allow 3 fields of premises

* refactor to allow 3 fields

* ignore unindexed local_premises

* update tests, include mepo improved

* add getIndexedImportedPremises

* refactor: not use module name as identifiers

* typo

* misc changes

* bump lean to 4.18

* limit max new premises to 512

* downsize model

* revert downsize

* robustify server

* typo

* server refactor using fastapi

* finish server refactor with test updates

* small refactors

* remove imported modules

* remove faiss-gpu

* increase max new premises

* minor

* legacy support for imported_modules

* legacy support for imported_modules

* update url to 4.18.0

* update downloading logic

* update url

* update url

* server wip

* use slim

* apt-get update

* bugfixes

* misc

* refactor concurrency

* bugfix & tune

* migrate server code to lean-premise-server

* remove dependency on Batteries

* add doc

* add module header

PremiseSelection/Cloud.lean
@@ -4,66 +4,204 @@ import PremiseSelection.Premise
 
 namespace Lean.PremiseSelection.Cloud
 
-register_option apiBaseUrl : String := {
-  defValue := "http://52.206.70.13"
+register_option premiseSelection.apiBaseUrl : String := {
+  defValue := "http://leanpremise.net"
   descr := "The base URL of the premise retrieval API"
 }
 
 def getApiBaseUrl (opts : Options) : String :=
-  apiBaseUrl.get opts
+  premiseSelection.apiBaseUrl.get opts
+
+def makeRequest {α : Type _} [FromJson α] (method urlPath : String) (data? : Option Json) : CoreM α := do
+  let apiBaseUrl := getApiBaseUrl (← getOptions)
+  let apiUrl := apiBaseUrl ++ urlPath
+  let mut curlArgs := #[
+    "-X", method,
+    "--user-agent", "LeanProver (https://leanprover-community.github.io/)"
+  ]
+  if data?.isSome then
+    curlArgs := curlArgs ++ #[
+      "--header", "Content-Type: application/json",
+      -- We put data in stdin rather than command argument, because the data may be too long
+      "--data", "@-"
+    ]
+  curlArgs := curlArgs.push apiUrl
+
+  let output : IO.Process.Output ← id <| do
+    if let some data := data? then
+      let childInit ← IO.Process.spawn { cmd := "curl", args := curlArgs, stdin := .piped, stdout := .piped, stderr := .piped }
+      let (stdin, child) ← childInit.takeStdin
+      stdin.putStr data.compress
+      let exitCode ← child.wait
+      let stdout ← child.stdout.readToEnd
+      let stderr ← child.stderr.readToEnd
+      return { exitCode, stdout, stderr }
+    else
+      IO.Process.output { cmd := "curl", args := curlArgs }
+
+  if output.exitCode != 0 then
+    IO.throwServerError <|
+      s!"Could not send API request to {apiUrl}. " ++
+      s!"curl exited with code {output.exitCode}:\n{output.stderr}"
+
+  match Json.parse output.stdout >>= fromJson? with
+  | .ok (result : α) =>
+      return result
+  | .error e => IO.throwServerError <|
+      s!"Could not parse server output (error: {e})\nRaw output:\n{output.stdout}"
 
 section IndexedPremises
 
-/-! Retrieving indexed premises and modules stored on the server -/
+/-! Retrieving indexed premises and modules stored on the server, and collecting
+new premises either imported or defined locally.
 
-/-- Unfiltered list of all premises known by the server.
-This is currently not used in Lean (but the API `/indexed-premises` will always be available). -/
-def getIndexedPremises (apiBaseUrl : String) : IO NameSet := do
-  let apiUrl := apiBaseUrl ++ "/indexed-premises"
-  let curlArgs := #[
-    "-X", "GET",
-    "--user-agent", "LeanProver (https://leanprover-community.github.io/)",
-    apiUrl
-  ]
-  let out ← IO.Process.output { cmd := "curl", args := curlArgs }
+The reason we make the distinction between imported and local premises is only because
+we can cache the results (set of premises and their signatures if unindexed) for imported
+premises in `IO.Ref`, because they won't change unless imports are changed.
 
-  if out.exitCode != 0 then
-    IO.throwServerError <|
-      "Could not send API request to retrieve premises. " ++
-      s!"curl exited with code {out.exitCode}:\n{out.stderr}"
+Indexed premises are represented by a `Nat` (index in `getIndexedPremisesFromServer`).
+Unindexed premises are represented as a `Premise` (name and signature).
+-/
 
-  match Json.parse out.stdout >>= fromJson? with
-  | .ok (result : Array String) =>
-      let mut names := ∅
-      for name in result do
-        names := names.insert name.toName
-      return names
-  | .error e => IO.throwServerError <|
-      s!"Could not parse server output (error: {e})"
+/-- The maximum number of new premises to send to the server. -/
+def getMaxUnindexedPremises : CoreM Nat := do
+  makeRequest "GET" "/max-new-premises" none
 
-/-- All modules known by the server. -/
-def getIndexedModules (apiBaseUrl : String) : IO NameSet := do
-  let apiUrl := apiBaseUrl ++ "/indexed-modules"
-  let curlArgs := #[
-    "-X", "GET",
-    "--user-agent", "LeanProver (https://leanprover-community.github.io/)",
-    apiUrl
-  ]
-  let out ← IO.Process.output { cmd := "curl", args := curlArgs }
+/-- A cache holding indexed premises by the server. -/
+initialize indexedPremisesFromServerRef : IO.Ref (Option (NameMap Nat)) ← IO.mkRef none
+/-- Unfiltered list of all premises known by the server, as a mapping from name to index.
+The result is cached in an `IO.Ref`, because (assuming the server is static) the result will not change. -/
+def getIndexedPremisesFromServer : CoreM (NameMap Nat) := do
+  match ← indexedPremisesFromServerRef.get with
+  | some map => return map
+  | none =>
+    let map ← core
+    indexedPremisesFromServerRef.set (some map)
+    return map
+where
+  core : CoreM (NameMap Nat) := do
+    let names : Array String ← makeRequest "GET" "/indexed-premises" none
+    return names.zipIdx.foldl (fun ns (n, i) => ns.insert n.toName i) ∅
 
-  if out.exitCode != 0 then
-    IO.throwServerError <|
-      "Could not send API request to retrieve modules. " ++
-      s!"curl exited with code {out.exitCode}:\n{out.stderr}"
+/-- All modules known by the server. **NOTE** This is not used. -/
+def getIndexedModules : CoreM NameSet := do
+  let moduleNames : Array String ← makeRequest "GET" "/indexed-modules" none
+  return moduleNames.foldl (fun ns n => ns.insert n.toName) ∅
 
-  match Json.parse out.stdout >>= fromJson? with
-  | .ok (result : Array String) =>
-      let mut moduleNames := ∅
-      for moduleName in result do
-        moduleNames := moduleNames.insert moduleName.toName
-      return moduleNames
-  | .error e => IO.throwServerError <|
-      s!"Could not parse server output (error: {e})"
+/-- A cache holding the premises imported from other modules that are indexed by the server. -/
+initialize indexedImportedPremisesRef : IO.Ref (Option (Array Nat)) ← IO.mkRef none
+/-- A cache holding the premises imported from other modules that are not indexed by the server. -/
+initialize unindexedImportedPremisesRef : IO.Ref (Option (Array Premise)) ← IO.mkRef none
+
+/-- Get imported premises, separated by whether they are indexed by the server. -/
+protected def getImportedPremisesCore (chunkSize := 256) : CoreM (Array Nat × Array Premise) := do
+  let env ← getEnv
+  let maxUnindexedPremises ← getMaxUnindexedPremises
+  let indexedPremisesFromServer ← getIndexedPremisesFromServer
+  let moduleNames := env.header.moduleNames
+  let moduleData := env.header.moduleData
+
+  let mut indexedIdxs := #[]
+  let mut unindexedNames := #[]
+  for i in [0:moduleData.size] do
+    let moduleName := moduleNames[i]!
+    if isDeniedModule env moduleName then
+      continue
+    let modData := moduleData[i]!
+    for name in modData.constNames do
+      if let some idx := indexedPremisesFromServer.find? name then
+        indexedIdxs := indexedIdxs.push idx
+      else
+        unless isDeniedPremise env name do
+          unindexedNames := unindexedNames.push name
+
+  if unindexedNames.size > maxUnindexedPremises then
+    logWarning m!"Found {unindexedNames.size} unindexed premises in imports, which exceeds the maximum number of new premises ({maxUnindexedPremises}). Discarding premises beyond this limit"
+    unindexedNames := unindexedNames.extract (unindexedNames.size - maxUnindexedPremises)
+  -- `useCache := false` because the `Premise`s are cached using our `unindexedImportedPremisesRef`
+  let unindexedPremises ← Premise.fromNames unindexedNames chunkSize false
+
+  return (indexedIdxs, unindexedPremises)
+
+/-- Get the imported premises that are indexed by the server. The result is cached in an `IO.Ref`,
+because (assuming the server is static) the result will not change unless the file is restarted. -/
+def getIndexedImportedPremises (chunkSize := 256) : CoreM (Array Nat) := do
+  match ← indexedImportedPremisesRef.get with
+  | some idxs => return idxs
+  | none =>
+    let (idxs, _) ← Cloud.getImportedPremisesCore chunkSize
+    indexedImportedPremisesRef.set (some idxs)
+    return idxs
+
+/-- Get the imported premises not indexed by the server. The result is cached in an `IO.Ref`,
+because (assuming the server is static) the result will not change unless the file is restarted. -/
+def getUnindexedImportedPremises (chunkSize := 256) : CoreM (Array Premise) := do
+  match ← unindexedImportedPremisesRef.get with
+  | some premises => return premises
+  | none =>
+    let (_, premises) ← Cloud.getImportedPremisesCore chunkSize
+    unindexedImportedPremisesRef.set (some premises)
+    return premises
+
+/-- Get the local premises defined in the current file that are indexed by the server.
+Modifications to these premises will *not* be reflected in the retrieval results, with
+the assumption being even if modifications are made, they should be small enough
+to significantly change the semantic meaning (the name is kept after all).
+-/
+def getIndexedLocalPremises : CoreM (Array Nat) := do
+  let env ← getEnv
+  let indexedPremisesFromServer ← getIndexedPremisesFromServer
+  let mut idxs := #[]
+  for (name, _) in env.constants.map₂ do
+    if let some idx := indexedPremisesFromServer.find? name then
+      idxs := idxs.push idx
+  return idxs
+
+/-- Returns the local premises defined in the current file that are not indexed by the server.
+The set of premises is not cached, to allow for adding/deleting local premises (unless indexed by the server).
+Currently, the printed signature itself is cached by the `Premise.fromName` function,
+meaning that it does not support modifying local premises,
+but (**TODO**) this behavior might (or should) change in the future by disabling this cache.
+-/
+def getUnindexedLocalPremises (chunkSize := 256) : CoreM (Array Premise) := do
+  let env ← getEnv
+  let indexedPremisesFromServer ← getIndexedPremisesFromServer
+  let mut names := #[]
+  for (name, _) in env.constants.map₂ do
+    unless indexedPremisesFromServer.contains name do
+      unless isDeniedPremise env name do
+        names := names.push name
+  Premise.fromNames names chunkSize true -- **TODO** see docstring
+
+/-- Returns new unindexed premises defined in the environment, from both imported and local premises,
+truncated to the maximum number of unindexed premises allowed by the server. -/
+def getUnindexedPremises (chunkSize := 256) : CoreM (Array Premise) := do
+  let maxUnindexedPremises ← getMaxUnindexedPremises
+  let premises₁ ← getUnindexedImportedPremises chunkSize
+  let premises₂ ← getUnindexedLocalPremises chunkSize
+  let mut premises := premises₁ ++ premises₂
+  if premises.size > maxUnindexedPremises then
+    -- This log message is not accurate because premises₁ is already truncated
+    -- logWarning m!"Found {premises.size} unindexed premises in the environment, which exceeds the maximum number of new premises ({maxUnindexedPremises}). Discarding premises beyond this limit"
+    premises := premises.extract (premises.size - maxUnindexedPremises)
+  return premises.extract (premises.size - maxUnindexedPremises) premises.size
+
+/-- Returns indexed premises defined in the environment, from both imported and local premises. -/
+def getIndexedPremises (chunkSize := 256) : CoreM (Array Nat) := do
+  let idxs₁ ← getIndexedImportedPremises chunkSize
+  let idxs₂ ← getIndexedLocalPremises
+  return idxs₁ ++ idxs₂
+
+elab "set_premise_selection_cloud_cache" : command => do
+  Elab.Command.liftCoreM do
+    let _ ← getUnindexedPremises
+    let _ ← getIndexedPremises
+
+elab "clear_premise_selection_cloud_cache" : command => do
+  Premise.fromNameCacheRef.set ∅
+  indexedPremisesFromServerRef.set none
+  indexedImportedPremisesRef.set none
+  unindexedImportedPremisesRef.set none
 
 end IndexedPremises
 
@@ -81,54 +219,34 @@ scoped instance : ToMessageData Suggestion where
 
 initialize Lean.registerTraceClass `premiseSelection.debug
 
-def selectPremisesCore (apiBaseUrl : String) (state : String)
-    (importedModules : Option (Array Name)) (newPremises : Option (Array Premise))
-    (k : Nat) : IO (Array Suggestion) := do
-  let apiUrl := apiBaseUrl ++ "/retrieve"
+def selectPremisesCore (state : String)
+    (indexedPremises : Array Nat) (unindexedPremises : Array Premise)
+    (k : Nat) : CoreM (Array Suggestion) := do
   let data := Json.mkObj [
     ("state", .str state),
-    ("imported_modules", toJson importedModules),
-    ("new_premises", toJson newPremises),
+    ("local_premises", toJson indexedPremises),  -- the name `local_premises` is an artifact from previous versions
+    ("new_premises", toJson unindexedPremises),
     ("k", .num (.fromNat k)),
   ]
-  let curlArgs := #[
-    "-X", "POST",
-    "--header", "Content-Type: application/json",
-    "--user-agent", "LeanProver (https://leanprover-community.github.io/)",
-    "--data-raw", data.compress,
-    apiUrl
-  ]
-  let out ← IO.Process.output { cmd := "curl", args := curlArgs }
-
-  if out.exitCode != 0 then
-    IO.throwServerError <|
-      "Could not send API request to select premises. " ++
-      s!"curl exited with code {out.exitCode}:\n{out.stderr}"
-
-  match Json.parse out.stdout >>= fromJson? with
-  | .ok result => return result
-  | .error e => IO.throwServerError <|
-      s!"Could not parse premise retrieval output (error: {e})\nRaw output:\n{out.stdout}"
+  makeRequest "POST" "/retrieve" (some data)
 
 def selectPremises (goal : MVarId) (k : Nat) : MetaM (Array Suggestion) := do
-  let env ← getEnv
+  -- let env ← getEnv
   let state ← withOptions (fun o => (o.set `pp.notation false).set `pp.fullNames true) $ Meta.ppGoal goal
   let state := state.pretty
   trace[premiseSelection.debug] m!"State: {state}"
 
-  let importedModules := env.allImportedModuleNames
-  let indexedModules ← getIndexedModules (getApiBaseUrl (← getOptions))
-  let newPremises ← Premise.getPremises indexedModules
-  let apiBaseUrl := getApiBaseUrl (← getOptions)
+  let indexedPremises ← getIndexedPremises
+  let unindexedPremises ← getUnindexedPremises
 
   let suggestions ← profileitM Exception "Cloud.selectPremises" (← getOptions) do
-    selectPremisesCore apiBaseUrl state importedModules newPremises k
+    selectPremisesCore state indexedPremises unindexedPremises k
 
   trace[premiseSelection.debug] m!"Suggestions: {suggestions}"
   return suggestions
 
 def premiseSelector : Selector := fun goal config => do
-  let premises ← selectPremises goal (config.maxSuggestions.getD 16)
+  let premises ← selectPremises goal (config.maxSuggestions.getD 32)
   premises.filterM fun suggestion => config.filter suggestion.name
 
 end Lean.PremiseSelection.Cloud
