PremiseSelection.lean
@@ -1,3 +1,4 @@
 import PremiseSelection.Basic
 import PremiseSelection.Cloud
+import PremiseSelection.MePo
 import PremiseSelection.Premise
