PremiseSelection/Basic.lean
@@ -1,0 +1,53 @@
+/-
+Copyright (c) 2025 Lean FRO, LLC. All rights reserved.
+Released under Apache 2.0 license as described in the file LICENSE.
+Authors: Kim Morrison, Thomas Zhu
+
+(This file is copied from the `mepo` branch in `leanprover/lean4`.)
+-/
+import Lean.PremiseSelection
+
+namespace Lean.PremiseSelection
+
+section DenyList
+
+/-- Premises from a module whose name has one of the following components are not retrieved. -/
+initialize moduleDenyListExt : SimplePersistentEnvExtension String (List String) ←
+  registerSimplePersistentEnvExtension {
+    addEntryFn := (·.cons)
+    addImportedFn := mkStateFromImportedEntries (·.cons) []
+  }
+
+/-- A premise whose name has one of the following components is not retrieved. -/
+initialize nameDenyListExt : SimplePersistentEnvExtension String (List String) ←
+  registerSimplePersistentEnvExtension {
+    addEntryFn := (·.cons)
+    addImportedFn := mkStateFromImportedEntries (·.cons) []
+  }
+
+/-- A premise whose `type.getForallBody.getAppFn` is a constant that has one of these prefixes is not retrieved. -/
+initialize typePrefixDenyListExt : SimplePersistentEnvExtension Name (List Name) ←
+  registerSimplePersistentEnvExtension {
+    addEntryFn := (·.cons)
+    addImportedFn := mkStateFromImportedEntries (·.cons) []
+  }
+
+def isDeniedModule (env : Environment) (moduleName : Name) : Bool :=
+  (moduleDenyListExt.getState env).any fun p => moduleName.anyS (· == p)
+
+def isDeniedPremise (env : Environment) (name : Name) : Bool := Id.run do
+  if name == ``sorryAx then return true
+  if name.isInternalDetail then return true
+  if (nameDenyListExt.getState env).any (fun p => name.anyS (· == p)) then return true
+  if let some moduleIdx := env.getModuleIdxFor? name then
+    let moduleName := env.header.moduleNames[moduleIdx.toNat]!
+    if isDeniedModule env moduleName then
+      return true
+  let some ci := env.find? name | return true
+  if let .const fnName _ := ci.type.getForallBody.getAppFn then
+    if (typePrefixDenyListExt.getState env).any (fun p => p.isPrefixOf fnName) then return true
+  return false
+
+end DenyList
+
+end Lean.PremiseSelection
