PremiseSelectionTest.lean
@@ -1,6 +1,9 @@
 import PremiseSelection
+import Lean
 
 open Lean PremiseSelection
+
+set_option trace.premiseSelection.debug true
 
 section Cloud
 
@@ -13,11 +16,37 @@ theorem add_comm (a b : Nat) : a + b = b + a := Nat.add_comm ..
 theorem Nat.add.comm (a b : Nat) : a + b = b + a := Nat.add_comm ..
 
 set_premise_selector premiseSelector
+set_option premiseSelection.apiBaseUrl "http://leanpremise.net"
 
 section Profiling
 
 set_option profiler true
 
+section ClientSideCache
+
+#time  -- populate cache for premises to send to server
+set_premise_selection_cloud_cache
+
+#time  -- second call to cache; should be fast
+set_premise_selection_cloud_cache
+
+end ClientSideCache
+
+section ServerSideCache
+
+#time  -- first server call
+example : True := by
+  suggest_premises
+  trivial
+
+#time  -- second server call (to test server-side caching; need a freshly started server)
+example : True := by
+  suggest_premises
+  trivial
+
+end ServerSideCache
+
+#time
 example (a b : Nat) : a + b = b + a := by
   suggest_premises
   apply Nat.add_comm
@@ -25,92 +54,69 @@ example (a b : Nat) : a + b = b + a := by
 -- The output is nonsense if no imported module and local premise information is provided
 -- (i.e. no premise to select from)
 #eval show CoreM _ from do
-  let url := getApiBaseUrl (← getOptions)
-  selectPremisesCore url "a b : Nat
-    ⊢ Eq (HAdd.hAdd a b) (HAdd.hAdd b a)" none none 2
+  selectPremisesCore "a b : Nat
+    ⊢ Eq (HAdd.hAdd a b) (HAdd.hAdd b a)" #[] #[] 2
 
 #eval show CoreM _ from do
-  let url := getApiBaseUrl (← getOptions)
-  selectPremisesCore url "a b : Nat
-    ⊢ Eq (HAdd.hAdd a b) (HAdd.hAdd b a)" none (some #[← Premise.fromName ``Nat.add.comm]) 2
-
-end Profiling
-
-set_option trace.premiseSelection.debug true
+  selectPremisesCore "a b : Nat
+    ⊢ Eq (HAdd.hAdd a b) (HAdd.hAdd b a)" #[] #[← Premise.fromName ``Nat.add.comm false] 2
 
 elab "simp_all_premises" k:num : tactic => do
-  let suggestions ← selectPremises (← Elab.Tactic.getMainGoal) k.getNat
+  let suggestions ← select (← Elab.Tactic.getMainGoal) { maxSuggestions := k.getNat }
   let simpLemmas : Array (TSyntax `Lean.Parser.Tactic.simpLemma) ←
     suggestions.mapM fun suggestion => do
-      let name := ⟨(mkIdent suggestion.name).raw⟩
+      let name := mkIdent suggestion.name
       `(Lean.Parser.Tactic.simpLemma| $name:term)
   Elab.Tactic.evalTactic (← `(tactic| simp_all [$simpLemmas,*]))
 
+#time
 example (a b : Nat) : a + b = b + a := by
   simp_all_premises 16
 
+#time
 example (a b : Nat) : a + (b + 1) = (a + b) + 1 := by
   simp_all_premises 16
 
+#time
+example (a b : Nat) : a + (b + 1) = (a + b) + 1 := by
+  simp_all_premises 16
+
+end Profiling
+
 end Cloud
 
--- Check the legacy API works
-
-deriving instance FromJson for Suggestion in
-def callApiLegacy (apiBaseUrl : String) (state : String)
-    (importedModules : Option (Array Name)) (newPremises : Option (Array Name))
-    (k : Nat) : IO (Array Suggestion) := do
-  let apiUrl := apiBaseUrl ++ "/retrieve"
-  let data := Json.mkObj [
-    ("state", .str state),
-    ("imported_modules", toJson importedModules),
-    ("local_premises", toJson newPremises),
-    ("k", .num (.fromNat k)),
-  ]
-  let curlArgs := #[
-    "-X", "POST",
-    "--header", "Content-Type: application/json",
-    "--user-agent", "LeanProver (https://leanprover-community.github.io/)",
-    "--data-raw", data.compress,
-    apiUrl
-  ]
-  let out ← IO.Process.output { cmd := "curl", args := curlArgs }
-
-  if out.exitCode != 0 then
-    IO.throwServerError <|
-      "Could not send API request to select premises. " ++
-      s!"curl exited with code {out.exitCode}:\n{out.stderr}"
-
-  match Json.parse out.stdout >>= fromJson? with
-  | .ok result => return result
-  | .error e => IO.throwServerError <|
-      s!"Could not parse premise retrieval output (error: {e})\nRaw output:\n{out.stdout}"
-
-deriving instance Repr for Suggestion in
-#eval show CoreM _ from do
-  let baseUrl := Cloud.getApiBaseUrl (← getOptions)
-  callApiLegacy baseUrl "a b : Nat\n⊢ Eq (HAdd.hAdd a b) (HAdd.hAdd b a)" none #[``Nat.add_comm] 10
-
 section Premise
+
+#eval Cloud.getUnindexedImportedPremises
+#eval Cloud.getUnindexedLocalPremises
+#time
+#eval Cloud.getUnindexedPremises
+-- clear_premise_selection_cache
+#time
+#eval show CoreM _ from do
+  let premises ← Cloud.getIndexedPremises
+  let json := toJson premises
+  return json.compress.length
 
 /--
 info: { name := `Nat.add,
   decl := "/-- Addition of natural numbers.\n\nThis definition is overridden in both the kernel and the compiler to efficiently\nevaluate using the \"bignum\" representation (see `Nat`). The definition provided\nhere is the logical model (and it is soundness-critical that they coincide).\n -/\ndef Nat.add : Nat → Nat → Nat" }
 -/
-#guard_msgs in #eval Premise.fromName ``Nat.add
+#guard_msgs in #eval Premise.fromName ``Nat.add false
 
 /--
 info: { name := `Nat.add_comm, decl := "theorem Nat.add_comm (n m : Nat) : Eq (HAdd.hAdd n m) (HAdd.hAdd m n)" }
 -/
-#guard_msgs in #eval Premise.fromName ``Nat.add_comm
-
-#eval show MetaM _ from do
-  let names ← Premise.getNames (← Cloud.getIndexedModules (Cloud.getApiBaseUrl (← getOptions)))
-  assert! names.contains ``add_comm_nat
-  IO.eprintln (names.take 100)
+#guard_msgs in #eval Premise.fromName ``Nat.add_comm false
 
 -- set_option profiler true
 -- set_option profiler.threshold 1
+
+-- #time
+-- #eval show MetaM _ from do
+--   let env ← getEnv
+--   for (name, ci) in env.constants do
+--     discard $ Premise.fromName name
 
 -- #eval show IO _ from do
 --   let cache ← Premise.fromNameCacheRef.get
@@ -119,10 +125,10 @@ info: { name := `Nat.add_comm, decl := "theorem Nat.add_comm (n m : Nat) : Eq (H
 
 section Generated
 
-/-! Generate 10000 theorems -/
+/-! Generate 1000 theorems -/
 
 #eval show Elab.Command.CommandElabM _ from do
-  for i in [0:10000] do
+  for i in [0:1000] do
     let name : Name := .str (.str .anonymous "Generated") s!"theorem{i}"
     Elab.Command.elabCommand (← `(command| theorem $(mkIdent name) : $(Syntax.mkNatLit i) = $(Syntax.mkNatLit i) := rfl))
 
@@ -130,12 +136,34 @@ end Generated
 
 #time
 #eval show MetaM _ from do
-  let premises ← Premise.getPremises (← Cloud.getIndexedModules (Cloud.getApiBaseUrl (← getOptions)))
-  assert! 10000 <= premises.size && premises.size < 20000
-  return premises.size
+  let premises ← Cloud.getUnindexedLocalPremises
+  assert! 1000 <= premises.size && premises.size < 2000
+  return premises
 
--- This makes the server OOM
--- example : 4882 = 4882 := by
---   suggest_premises
+-- This makes the server OOM if not for maxUnindexedPremises
+example : 4882 = 4882 := by
+  suggest_premises
+  rfl
+
+-- Stress test
+-- #eval show MetaM _ from do
+--   let premises : Array Premise := (Array.range 500).map fun n =>
+--     { name := s!"thm{n}".toName, decl := "theorem MeasureTheory.pdf.indepFun_iff_pdf_prod_eq_pdf_mul_pdf {Ω : Type u_1} {E : Type u_2} [MeasurableSpace E] {m : MeasurableSpace Ω} {ℙ : Measure Ω} {μ : Measure E} {F : Type u_3} [MeasurableSpace F] {ν : Measure F} {X : Ω → E} {Y : Ω → F} [IsFiniteMeasure ℙ] [SigmaFinite μ] [SigmaFinite ν] [HasPDF (fun (ω : Ω) => (X ω, Y ω)) ℙ (μ.prod ν)] : ProbabilityTheory.IndepFun X Y ℙ ↔ pdf (fun (ω : Ω) => (X ω, Y ω)) ℙ (μ.prod ν) =ᶠ[ae (μ.prod ν)] fun (z : E × F) => pdf X ℙ μ z.1 * pdf Y ℙ ν z.2" }
+--   Cloud.selectPremisesCore "a b : Nat ⊢ Eq (HAdd.hAdd a b) (HAdd.hAdd b a)" #[] #[] premises 32
 
 end Premise
+
+section MePo
+
+open MePo
+
+def mepoP := 0.6
+def mepoC := 0.9
+
+set_premise_selector mepoSelector (useRarity := true) (p := mepoP) (c := mepoC)
+
+example (a b : Nat) : a + b = b + a := by
+  suggest_premises
+  simp_all_premises 16
+
+end MePo
